CopySymbols_L

TM/Compound/CopySymbols.v
@@ -262,7 +262,134 @@ End Test.
 
   Definition CopySymbols_L := Mirror CopySymbols.
 
+  Definition llength (t : tape sig) :=
+    match t with
+    | midtape ls m rs => 1 + length ls
+    | _ => 0
+    end.
+
+  Definition llength' (tin : tape sig * tape sig) : nat := llength (fst tin).
+
+  Function CopySymbols_L_Fun (tin : tape sig * tape sig) { measure llength' tin } : tape sig * tape sig :=
+    match tin with
+      (midtape ls m rs as t1, t2) =>
+      if f m
+      then (t1, tape_write t2 (Some (g m)))
+      else CopySymbols_L_Fun (tape_move_left t1, tape_move_mono t2 (Some (g m), L))
+    | (t1, t2) => (t1, t2)
+    end.
+  Proof.
+    all: (intros; try now (cbn; omega)).
+    destruct ls; cbn. omega. omega.
+  Qed.
+
+
+  Lemma CopySymbols_mirror t t' :
+    CopySymbols_Fun (mirror_tape (fst t), mirror_tape (snd t)) =
+    (mirror_tape (fst t'), mirror_tape (snd t')) ->
+    CopySymbols_L_Fun t = t'.
+  Proof.
+    functional induction CopySymbols_L_Fun t; intros H; cbn in *; try reflexivity;
+      rewrite CopySymbols_Fun_equation in H; cbn; auto.
+    - rewrite e0 in H. cbn in *.
+      destruct t' as (t1',t2'); cbn in *. inv H.
+      apply mirror_tape_inv_midtape in H1. subst.
+      apply mirror_tape_inv_midtape in H2. subst.
+      simpl_tape. reflexivity.
+    - rewrite e0 in H. cbn in *.
+      destruct t' as (t1',t2'); cbn in *.
+      destruct ls; cbn in *; simpl_tape in *.
+      + rewrite CopySymbols_Fun_equation in H. inv H.
+        apply mirror_tape_inv_rightof in H1. subst.
+        eapply IHp; clear IHp. rewrite CopySymbols_Fun_equation. f_equal. f_equal.
+        destruct (left t2); cbn.
+        * apply mirror_tape_inv_rightof in H2. subst. reflexivity.
+        * apply mirror_tape_inv_midtape in H2. subst. reflexivity.
+      + eapply IHp; clear IHp. rewrite <- H; clear H.
+        f_equal. f_equal.
+        destruct (left t2); cbn; auto.
+    - destruct t' as (t1',t2'). destruct t1; cbn in *; inv H; auto.
+      1: apply mirror_tape_inv_niltape in H1.
+      2: apply mirror_tape_inv_rightof in H1.
+      3: apply mirror_tape_inv_leftof in H1.
+      all: apply mirror_tape_injective in H2.
+      all: congruence.
+  Qed.
+
+
+  Lemma CopySymbols_mirror' t t' :
+    CopySymbols_L_Fun (mirror_tape (fst t), mirror_tape (snd t)) =
+    (mirror_tape (fst t'), mirror_tape (snd t')) ->
+    CopySymbols_Fun t = t'.
+  Proof.
+    functional induction CopySymbols_Fun t; intros H; cbn in *; try reflexivity;
+      rewrite CopySymbols_L_Fun_equation in H; cbn; auto.
+    - rewrite e0 in H. inv H.
+      destruct t' as (t1',t2'). cbn in *.
+      apply mirror_tape_inv_midtape in H1.
+      apply mirror_tape_inv_midtape in H2.
+      subst. simpl_tape. reflexivity.
+    - rewrite e0 in H.
+      destruct t' as (t1',t2'). cbn in *.
+      eapply IHp; clear IHp. rewrite <- H; clear H.
+      f_equal. f_equal; simpl_tape.
+      + destruct rs; cbn; reflexivity.
+      + destruct (right t2); cbn; reflexivity.
+    - destruct t' as (t1',t2'). cbn in *.
+      destruct t1; cbn in *; inv H; auto.
+      1: apply mirror_tape_inv_niltape in H1.
+      2: apply mirror_tape_inv_rightof in H1.
+      3: apply mirror_tape_inv_leftof in H1.
+      all: apply mirror_tape_injective in H2.
+      all: congruence.
+  Qed.
+
+
+  Definition CopySymbols_L_Rel : Rel (tapes sig 2) (unit * tapes sig 2) :=
+    ignoreParam (fun tin tout => ((tout[@Fin.F1], tout[@Fin.FS Fin.F1]) = CopySymbols_L_Fun (tin[@Fin.F1], tin[@Fin.FS Fin.F1]))).
+
+  Lemma CopySymbols_L_WRealise : CopySymbols_L ⊫ CopySymbols_L_Rel.
+  Proof.
+    eapply WRealise_monotone.
+    { eapply Mirror_WRealise. eapply CopySymbols_WRealise. }
+    { intros tin ((), tout) H. cbn in *.
+      symmetry in H; symmetry. simpl_tape in H.
+      apply CopySymbols_mirror; eauto.
+    }
+  Qed.
+
   
+  Function CopySymbols_L_TermTime (t : tape sig) { measure llength t } : nat :=
+    match t with
+    | midtape ls m rs => if f m then 8 else 8 + CopySymbols_L_TermTime (tape_move_left t)
+    | _ => 8
+    end.
+  Proof.
+    all: (intros; try now (cbn; omega)). destruct ls; cbn; omega.
+  Qed.
+
+  
+  Lemma CopySymbols_TermTime_mirror t :
+    CopySymbols_L_TermTime t = CopySymbols_TermTime (mirror_tape t).
+  Proof.
+    functional induction CopySymbols_L_TermTime t; cbn; auto;
+      simpl_tape in *; cbn in *;
+        rewrite CopySymbols_TermTime_equation.
+    - now rewrite e0.
+    - now rewrite e0, IHn.
+    - destruct t; cbn; auto.
+  Qed.
+
+  Lemma CopySymbols_L_terminates :
+    projT1 CopySymbols_L ↓ (fun tin k => CopySymbols_L_TermTime (tin[@Fin.F1]) <= k).
+  Proof.
+    eapply TerminatesIn_monotone.
+    - eapply Mirror_Terminates. eapply CopySymbols_terminates.
+    - cbn. intros tin k Hk. destruct_tapes; cbn. rewrite <- Hk. unfold mirror_tapes.
+      rewrite CopySymbols_TermTime_mirror. cbn. auto.
+  Qed.
+  
+
 End CopySymbols.
 
 
@@ -270,6 +397,8 @@ Ltac smpl_TM_CopySymbols :=
   match goal with
   | [ |- CopySymbols  _ _ ⊫ _ ] => eapply CopySymbols_WRealise
   | [ |- projT1 (CopySymbols _ _) ↓ _ ] => eapply CopySymbols_terminates
+  | [ |- CopySymbols_L  _ _ ⊫ _ ] => eapply CopySymbols_L_WRealise
+  | [ |- projT1 (CopySymbols_L _ _) ↓ _ ] => eapply CopySymbols_L_terminates
   end.
 
 Smpl Add smpl_TM_CopySymbols : TM_Correct.
